Negatively solved

PromiseCombinators.thy
@@ -5,6 +5,7 @@ datatype expr =
   Num nat |
   Tuple expr expr |
   Pending expr expr |
+  PendingForever |
   Resolve expr |
   Reject expr |
   All2 expr |
@@ -13,28 +14,35 @@ datatype expr =
 
 datatype event =
   EventResolve expr |
-  EventReject expr |
-  EventAll2 |
-  EventRace2L |
-  EventRace2R
-
+  EventReject expr
 
 
 text "Unfailable world"
 inductive
   UF_small_step :: "expr \<times> event list \<Rightarrow> expr \<times> event list \<Rightarrow> bool" (infix "\<Rightarrow>" 55)
 where
-  UF_NumNumI[intro]:         "(Num n, ev) \<Rightarrow> (Num n, ev)" |
-  UF_PendingResolveI[intro]: "(Pending a b, ev) \<Rightarrow> (Resolve a, ev@[EventResolve x])" |
-  UF_All2ResolveI[intro]:    "\<lbrakk> (All2 (Tuple a b), ev) \<Rightarrow> (All2 (Tuple (Resolve a') (Resolve b')), ev') \<rbrakk> \<Longrightarrow> (All2 (Tuple a b), ev) \<Rightarrow> (Resolve (Tuple a' b'), ev'@[EventAll2])" |
-  UF_Race2ResolveI1[intro]:  "\<lbrakk> (Race2 (Tuple a b), ev) \<Rightarrow> (Race2 (Tuple (Resolve a') _), ev') \<rbrakk> \<Longrightarrow> (Race2 (Tuple a b), ev) \<Rightarrow> (Resolve a', ev'@[EventRace2L])" |
-  UF_Race2ResolveI2[intro]:  "\<lbrakk> (Race2 (Tuple a b), ev) \<Rightarrow> (Race2 (Tuple _ (Resolve b')), ev') \<rbrakk> \<Longrightarrow> (Race2 (Tuple a b), ev) \<Rightarrow> (Resolve b', ev'@[EventRace2R])" |
+  UF_NumNumI[intro]:                "(Num n, ev) \<Rightarrow> (Num n, ev)" |
+  UF_PendingResolveI[intro]:        "(Pending a b, ev) \<Rightarrow> (Resolve a, ev@[EventResolve a])" |
+  UF_PendingPendingForeverI[intro]: "(Pending a b, ev) \<Rightarrow> (PendingForever, ev)" |
+  UF_PendingForeverPendingForeverI[intro]: "(PendingForever, ev) \<Rightarrow> (PendingForever, ev)" |
+  UF_All2ResolveI[intro]:           "\<lbrakk> (All2 (Tuple a b), ev) \<Rightarrow> (All2 (Tuple (Resolve a') (Resolve b')), ev') \<rbrakk> \<Longrightarrow> (All2 (Tuple a b), ev) \<Rightarrow> (Resolve (Tuple a' b'), ev')" |
+  UF_Race2ResolveI1[intro]:         "\<lbrakk> (Race2 (Tuple a b), ev) \<Rightarrow> (Race2 (Tuple (Resolve a') b'), ev') \<rbrakk> \<Longrightarrow> (Race2 (Tuple a b), ev) \<Rightarrow> (Resolve a', ev')" |
+  UF_Race2ResolveI2[intro]:         "\<lbrakk> (Race2 (Tuple a b), ev) \<Rightarrow> (Race2 (Tuple a' (Resolve b')), ev') \<rbrakk> \<Longrightarrow> (Race2 (Tuple a b), ev) \<Rightarrow> (Resolve b', ev')" |
 
-  UF_TupleTupleI[intro]:     "\<lbrakk> (a, ev) \<Rightarrow> (a', evA'); (b, ev) \<Rightarrow> (b', evB'); interleave evA' evB' ev' \<rbrakk> \<Longrightarrow> (Tuple a b, ev) \<Rightarrow> (Tuple a' b', ev')" |
-  UF_PendingPendingI[intro]: "\<lbrakk> (a, ev) \<Rightarrow> (a', evA'); (b, ev) \<Rightarrow> (b', evB'); interleave evA' evB' ev' \<rbrakk> \<Longrightarrow> (Pending a b, ev) \<Rightarrow> (Pending a' b', ev')" |
-  UF_ResolveResolveI[intro]: "\<lbrakk> (x, ev) \<Rightarrow> (x', ev') \<rbrakk> \<Longrightarrow> (Resolve x, ev) \<Rightarrow> (Resolve x', ev')" |
-  UF_All2All2I[intro]:       "\<lbrakk> (Tuple a b, ev) \<Rightarrow> (Tuple a' b', ev') \<rbrakk> \<Longrightarrow> (All2 (Tuple a b), ev) \<Rightarrow> (All2 (Tuple a' b'), ev')" |
-  UF_Race2Race2I[intro]:     "\<lbrakk> (Tuple a b, ev) \<Rightarrow> (Tuple a' b', ev') \<rbrakk> \<Longrightarrow> (Race2 (Tuple a b), ev) \<Rightarrow> (Race2 (Tuple a' b'), ev')"
+  UF_TupleTupleI[intro]:            "\<lbrakk> (a, ev) \<Rightarrow> (a', evA'); (b, ev) \<Rightarrow> (b', evB'); interleave evA' evB' ev' \<rbrakk> \<Longrightarrow> (Tuple a b, ev) \<Rightarrow> (Tuple a' b', ev')" |
+  UF_PendingPendingI[intro]:        "\<lbrakk> (a, ev) \<Rightarrow> (a', evA'); (b, ev) \<Rightarrow> (b', evB'); interleave evA' evB' ev' \<rbrakk> \<Longrightarrow> (Pending a b, ev) \<Rightarrow> (Pending a' b', ev')" |
+  UF_ResolveResolveI[intro]:        "\<lbrakk> (x, ev) \<Rightarrow> (x', ev') \<rbrakk> \<Longrightarrow> (Resolve x, ev) \<Rightarrow> (Resolve x', ev')" |
+  UF_All2All2I[intro]:              "\<lbrakk> (Tuple a b, ev) \<Rightarrow> (Tuple a' b', ev') \<rbrakk> \<Longrightarrow> (All2 (Tuple a b), ev) \<Rightarrow> (All2 (Tuple a' b'), ev')" |
+  UF_Race2Race2I[intro]:            "\<lbrakk> (Tuple a b, ev) \<Rightarrow> (Tuple a' b', ev') \<rbrakk> \<Longrightarrow> (Race2 (Tuple a b), ev) \<Rightarrow> (Race2 (Tuple a' b'), ev')"
+
+
+inductive_cases UF_All2_ResolveE: "(All2 (Tuple a b), ev) \<Rightarrow> (Resolve (Tuple a' b'), ev')"
+inductive_cases UF_All2_All2E: "(All2 (Tuple a b), ev) \<Rightarrow> (All2 (Tuple a' b'), ev')"
+inductive_cases UF_Tuple_TupleE: "(Tuple a b, ev) \<Rightarrow> (Tuple a' b', ev')"
+inductive_cases UF_Pending_ResolveE: "(Pending a b, ev) \<Rightarrow> (Resolve a', ev')"
+inductive_cases UF_Race2_ResolveE: "(Race2 (Tuple a b), ev) \<Rightarrow> (Resolve a', ev')"
+inductive_cases UF_Race2_Race2E: "(Race2 (Tuple a b), ev) \<Rightarrow> (Race2 (Tuple a' b'), ev')"
+inductive_cases UF_PendingForever_FreeE: "(PendingForever, ev) \<Rightarrow> (x', ev')"
 
 
 lemma "(Tuple (Num 0) (Num 1), []) \<Rightarrow> (Tuple (Num 0) (Num 1), [])"
@@ -52,7 +60,7 @@ lemma "(Pending (Num 0) (Num 1), []) \<Rightarrow> (Resolve (Num 0), [EventResol
   done
 
 
-lemma "(Race2 (Tuple (Pending (Num 0) (Num 1)) (Pending (Num 2) (Num 3))), []) \<Rightarrow> (Resolve (Num 0), [EventResolve (Num 0)]@[EventRace2L])"
+lemma "(Race2 (Tuple (Pending (Num 0) (Num 1)) (Pending (Num 2) (Num 3))), []) \<Rightarrow> (Resolve (Num 0), [EventResolve (Num 0)])"
   apply(rule UF_Race2ResolveI1)
   apply(rule UF_Race2Race2I)
   apply(subst (2) append.right_neutral[symmetric])
@@ -68,7 +76,7 @@ lemma "(Race2 (Tuple (Pending (Num 0) (Num 1)) (Pending (Num 2) (Num 3))), []) \
   done
 
 
-lemma "(Race2 (Tuple (Pending (Num 0) (Num 1)) (Pending (Num 2) (Num 3))), []) \<Rightarrow> (Resolve (Num 2), [EventResolve (Num 2)]@[EventRace2R])"
+lemma "(Race2 (Tuple (Pending (Num 0) (Num 1)) (Pending (Num 2) (Num 3))), []) \<Rightarrow> (Resolve (Num 2), [EventResolve (Num 2)])"
   apply(rule UF_Race2ResolveI2)
   apply(rule UF_Race2Race2I)
   apply(subst (2) append.right_neutral[symmetric])
@@ -84,8 +92,7 @@ lemma "(Race2 (Tuple (Pending (Num 0) (Num 1)) (Pending (Num 2) (Num 3))), []) \
   done
 
 
-lemma "(All2 (Tuple (Pending (Num 0) (Num 1)) (Pending (Num 2) (Num 3))), []) \<Rightarrow> (Resolve (Tuple (Num 0) (Num 2)), [EventResolve (Num 0)]@[EventResolve (Num 2)]@[EventAll2])"
-  apply(subst append_assoc[symmetric])
+lemma "(All2 (Tuple (Pending (Num 0) (Num 1)) (Pending (Num 2) (Num 3))), []) \<Rightarrow> (Resolve (Tuple (Num 0) (Num 2)), [EventResolve (Num 0)]@[EventResolve (Num 2)])"
   apply(rule UF_All2ResolveI)
   apply(rule UF_All2All2I)
   apply(rule_tac ev="[]" in UF_TupleTupleI)
@@ -96,8 +103,7 @@ lemma "(All2 (Tuple (Pending (Num 0) (Num 1)) (Pending (Num 2) (Num 3))), []) \<
   done
 
 
-lemma "(All2 (Tuple (Pending (Num 0) (Num 1)) (Pending (Num 2) (Num 3))), []) \<Rightarrow> (Resolve (Tuple (Num 0) (Num 2)), [EventResolve (Num 2)]@[EventResolve (Num 0)]@[EventAll2])"
-  apply(subst append_assoc[symmetric])
+lemma "(All2 (Tuple (Pending (Num 0) (Num 1)) (Pending (Num 2) (Num 3))), []) \<Rightarrow> (Resolve (Tuple (Num 0) (Num 2)), [EventResolve (Num 2)]@[EventResolve (Num 0)])"
   apply(rule UF_All2ResolveI)
   apply(rule UF_All2All2I)
   apply(rule_tac ev="[]" in UF_TupleTupleI)
@@ -107,14 +113,17 @@ lemma "(All2 (Tuple (Pending (Num 0) (Num 1)) (Pending (Num 2) (Num 3))), []) \<
   done
 
 
-fun flip :: "expr \<Rightarrow> expr" where
+fun
+  flip :: "expr \<Rightarrow> expr"
+where
   "flip (All2 a) = All2 (flip a)" |
   "flip (Race2 a) = Race2 (flip a)" |
   "flip (Tuple a b) = Tuple (flip b) (flip a)" |
   "flip (Pending a b) = Pending (flip a) (flip b)" |
   "flip (Resolve a) = Resolve (flip a)" |
   "flip (Reject a) = Reject (flip a)" |
-  "flip (Num n) = Num n"
+  "flip (Num n) = Num n" |
+  "flip PendingForever = PendingForever"
 
 
 theorem flip_self_inv: "self_inv flip"
@@ -125,21 +134,30 @@ theorem flip_self_inv: "self_inv flip"
   done
 
 
-fun flip_ev1 :: "event \<Rightarrow> event" where
-  "flip_ev1 EventRace2L = EventRace2R" |
-  "flip_ev1 EventRace2R = EventRace2L" |
-  "flip_ev1 x = x"
+lemma flip_flip_ident: "flip (flip x) = x"
+  apply(rule self_inv_self_inv_iff)
+  apply(rule flip_self_inv)
+  done
+
+
+fun
+  flip_ev1 :: "event \<Rightarrow> event"
+where
+  "flip_ev1 (EventResolve a) = EventResolve (flip a)" |
+  "flip_ev1 (EventReject b) = EventReject (flip b)"
 
 
 theorem flip_ev1_self_inv: "self_inv flip_ev1"
   apply(unfold self_inv_def)
   apply(clarify)
   apply(case_tac "x")
-  apply(auto)
+  apply(auto simp: self_inv_self_inv_iff flip_self_inv)
   done
 
 
-definition flip_ev :: "event list \<Rightarrow> event list" where
+definition
+  flip_ev :: "event list \<Rightarrow> event list"
+where
   "flip_ev \<equiv> map flip_ev1"
 
 
@@ -150,50 +168,246 @@ theorem flip_ev_self_inv: "self_inv flip_ev"
   done
 
 
-theorem UF_flip[rule_format]: "x \<Rightarrow> x' \<longrightarrow> (\<forall>e ev e' ev'. x = (e, ev) \<and> x' = (e', ev') \<longrightarrow> (flip e, flip_ev ev) \<Rightarrow> (flip e', flip_ev ev'))"
+lemma flip_ev_Nil: "flip_ev [] = []"
+  apply(unfold flip_ev_def)
+  apply(auto)
+  done
+
+
+lemma flip_ev_flip_ev_ident: "flip_ev (flip_ev x) = x"
+  apply(rule self_inv_self_inv_iff)
+  apply(rule flip_ev_self_inv)
+  done
+
+
+lemma UF_flipI[rule_format]: "x \<Rightarrow> x' \<longrightarrow> (\<forall>e ev e' ev'. x = (e, ev) \<and> x' = (e', ev') \<longrightarrow> (flip e, flip_ev ev) \<Rightarrow> (flip e', flip_ev ev'))"
   apply(rule impI)
   apply(erule UF_small_step.induct)
   apply(auto simp: flip_ev_def)
-  apply(force intro: interleave_mapI)
+  apply(rule UF_TupleTupleI)
+  apply(auto intro: interleave_mapI)
   apply(rule UF_PendingPendingI)
-  apply(assumption)
-  apply(assumption)
-  apply(rule interleave_mapI)
-  apply(subst interleave_flip)
-  apply(assumption)
+  apply(auto intro: interleave_mapI simp add: interleave_flip)
+  done
+
+
+lemma UF_flipD[rule_format]: "(flip x, flip_ev ev) \<Rightarrow> (flip x', flip_ev ev') \<longrightarrow> (x, ev) \<Rightarrow> (x', ev')"
+  apply(subgoal_tac "\<exists>y y' eev eev'. flip x = y \<and> flip x' = y' \<and> flip_ev ev = eev \<and> flip_ev ev' = eev' \<and> x = flip y \<and> x' = flip y' \<and> ev = flip_ev eev \<and> ev' = flip_ev eev'")
+  apply(elim exE conjE)
+  apply(erule ssubst)+
+  apply(rule impI)
+  apply(erule UF_flipI)
+  apply(auto simp add: flip_self_inv flip_ev_self_inv self_inv_self_inv_iff)
+  done
+
+
+theorem UF_flip: "(flip x, flip_ev ev) \<Rightarrow> (flip x', flip_ev ev') \<longleftrightarrow> (x, ev) \<Rightarrow> (x', ev')"
+  apply(rule iffI)
+  apply(erule UF_flipD)
+  apply(erule UF_flipI)
+  apply(simp)
   done
 
 
 theorem UF_arbitrariness: "\<exists>x0 x1 ev1 x2 ev2. (x0, []) \<Rightarrow> (x1, ev1) \<and> (x0, []) \<Rightarrow> (x2, ev2) \<and> x1 \<noteq> x2"
   apply(rule_tac x="Race2 (Tuple (Resolve (Num 1)) (Resolve (Num 2)))" in exI)
   apply(rule_tac x="Resolve (Num 1)" in exI)
-  apply(rule_tac x="[EventRace2L]" in exI)
+  apply(rule_tac x="[]" in exI)
   apply(rule_tac x="Resolve (Num 2)" in exI)
-  apply(rule_tac x="[EventRace2R]" in exI)
+  apply(rule_tac x="[]" in exI)
   apply(intro conjI)
   apply(subst (2) append.left_neutral[symmetric])
-  apply(rule)+
+  apply(rule UF_Race2ResolveI1)
+  apply(force)
   apply(subst (2) append.left_neutral[symmetric])
   apply(rule)+
-  apply(simp)
+  apply(auto)
   done
 
 
-definition Tuple3 :: "expr \<Rightarrow> expr \<Rightarrow> expr \<Rightarrow> expr" where
+definition
+  Tuple3 :: "expr \<Rightarrow> expr \<Rightarrow> expr \<Rightarrow> expr"
+where
   "Tuple3 a b c \<equiv> Tuple a (Tuple b c)"
 
 
-definition All3 :: "expr \<Rightarrow> expr \<Rightarrow> expr \<Rightarrow> expr" where
+definition
+  All3 :: "expr \<Rightarrow> expr \<Rightarrow> expr \<Rightarrow> expr"
+where
   "All3 a b c \<equiv> All2 (Tuple a (All2 (Tuple b c)))"
 
 
 theorem "\<exists>ev. (All3 (Pending (Num 3) (Num 0)) (Pending (Num 2) (Num 0)) (Pending (Num 1) (Num 0)), []) \<Rightarrow> (Resolve (Tuple3 (Num 3) (Num 2) (Num 1)), ev)"
-  apply(rule_tac x="[EventResolve (Num 3)]@[EventResolve (Num 2)]@[EventResolve (Num 1)]@[EventAll2]@[EventAll2]" in exI)
+  apply(rule_tac x="[EventResolve (Num 3)]@[EventResolve (Num 2)]@[EventResolve (Num 1)]" in exI)
   apply(unfold All3_def Tuple3_def)
   apply(subst append_assoc[symmetric])+
   apply(rule)+
   apply(force)
   apply(simp)
   apply(rule)+
+  done
+
+
+definition
+  events :: "expr \<Rightarrow> expr \<Rightarrow> event list set"
+where
+  "events x x' \<equiv> { ev | ev. (x, []) \<Rightarrow> (x', ev) }"
+
+
+lemma flip_Nil_flip_Free: "(flip x, []) \<Rightarrow> (flip x', ev) \<longleftrightarrow> (x, []) \<Rightarrow> (x', flip_ev ev)"
+  apply(subgoal_tac "\<exists>ev'. ev = flip_ev ev' \<and> ev' = flip_ev ev \<and> [] = flip_ev []")
+  apply(elim exE conjE)
+  apply(erule ssubst)+
+  apply(subst UF_flip)
+  apply(subst flip_ev_flip_ev_ident)
+  apply(subst flip_ev_Nil)
+  apply(rule refl)
+  apply(rule_tac x="flip_ev ev" in exI)
+  apply(force simp add: flip_ev_flip_ev_ident flip_ev_Nil)
+  done
+
+
+lemma events_flip_flip1[rule_format]: "\<lbrakk> fev = flip_ev ` events (flip x) (flip x') \<rbrakk> \<Longrightarrow> fev \<subseteq> events x x'"
+  apply(erule ssubst)
+  apply(unfold events_def)
+  apply(subst flip_Nil_flip_Free)
+  apply(auto simp add: image_def)
+  done
+
+
+lemma events_flip_flip2[rule_format]: "\<lbrakk> fev = flip_ev ` events (flip x) (flip x') \<rbrakk> \<Longrightarrow> events x x' \<subseteq> fev"
+  apply(subgoal_tac "\<exists>y y'. x = flip y \<and> x' = flip y'")
+  apply(elim exE conjE)
+  apply(erule ssubst)+
+  apply(simp only: flip_flip_ident)
+  apply(rule_tac x="flip_ev ` events (flip y) (flip y')" in self_inv_image_subsetI)
+  apply(rule flip_ev_self_inv)
+  apply(rule events_flip_flip1)
+  apply(rule refl)
+  apply(force simp add: flip_ev_flip_ev_ident)
+  apply(rule_tac x="flip x" in exI)
+  apply(rule_tac x="flip x'" in exI)
+  apply(force simp add: flip_flip_ident)
+  done
+
+
+lemma events_flip_flip: "flip_ev ` events (flip x) (flip x') = events x x'"
+  apply(rule equalityI)
+  apply(rule events_flip_flip1)
+  apply(rule refl)
+  apply(rule events_flip_flip2)
+  apply(rule refl)
+  done
+
+
+fun
+  to_appended_all :: "'a list \<Rightarrow> 'a list"
+where
+  "to_appended_all [] = []" |
+  "to_appended_all [x] = [x]" |
+  "to_appended_all (x1#x2#xs) = ([x1]@[x2])@(to_appended_all xs)"
+
+
+definition
+  appended_all :: "'a list \<Rightarrow> 'a list"
+where
+  "appended_all \<equiv> to_appended_all"
+
+
+lemma appended_all_map: "appended_all (map f x) = map f (appended_all x)"
+  apply(rule_tac P="\<lambda>x. appended_all (map f x) = map f (appended_all x)" in to_appended_all.induct)
+  apply(unfold appended_all_def flip_ev_def)
+  apply(auto)
+  done
+
+
+theorem All2_events: "
+  events
+    (All2 (Tuple (Pending (Num 1) (Num 0)) (Pending (Num 2) (Num 0))))
+    (Resolve (Tuple (Num 1) (Num 2)))
+  = {
+    appended_all [EventResolve (Num 1), EventResolve (Num 2)],
+    appended_all [EventResolve (Num 2), EventResolve (Num 1)]
+  }"
+  apply(unfold events_def)
+  apply(intro equalityI subsetI)
+  apply(clarsimp)
+  apply(elim UF_All2_ResolveE UF_All2_All2E UF_Tuple_TupleE UF_Pending_ResolveE)
+  apply(auto simp add: interleave_single_single)
+  apply(unfold appended_all_def to_appended_all.simps)
+  apply(force)
+  apply(force)
+  apply(rule)+
+  apply(simp add: interleave_single_single)
+  apply(rule)+
+  apply(simp add: interleave_single_single)
+  done
+
+
+theorem Race2L_events: "
+  events
+    (Race2 (Tuple (Pending (Num 1) (Num 0)) PendingForever))
+    (Resolve (Num 1))
+  = { appended_all [EventResolve (Num 1)] }"
+  apply(unfold events_def)
+  apply(intro equalityI subsetI)
+  apply(clarsimp)
+  apply(elim UF_Race2_ResolveE UF_Race2_Race2E UF_Tuple_TupleE UF_PendingForever_FreeE)
+  apply(clarsimp simp add: interleave_right_neutral)
+  apply(elim UF_Pending_ResolveE)
+  apply(force simp: appended_all_def)
+  apply(force)
+  apply(simp)
+  apply(clarify)
+  apply(unfold appended_all_def to_appended_all.simps append.right_neutral)
+  apply(rule UF_Race2ResolveI1)
+  apply(rule)+
+  apply(simp add: interleave_right_neutral)
+  done
+ 
+
+theorem Race2R_events: "
+  events
+    (Race2 (Tuple PendingForever (Pending (Num 1) (Num 0))))
+    (Resolve (Num 1))
+  = { appended_all [EventResolve (Num 1)] }"
+  apply(subst events_flip_flip[symmetric])
+  apply(subst self_inv_flip [where f="image flip_ev"])
+  apply(rule image_self_inv)
+  apply(rule flip_ev_self_inv)
+  apply(simp del: One_nat_def add: flip_ev_def appended_all_map[symmetric])
+  apply(rule Race2L_events)
+  done
+
+
+theorem "(
+  (Race2 (Tuple
+    (All2 (Tuple (Pending (Num 1) (Num 0)) (Pending (Num 1) (Num 0))))
+    (All2 (Tuple (Pending (Num 1) (Num 0)) PendingForever))
+  )), []) \<Rightarrow>
+  (Resolve (Tuple (Num 1) (Num 1)), [EventResolve (Num 1)]@[EventResolve (Num 1)])
+"
+  apply(rule UF_Race2ResolveI1)
+  apply(rule)+
+  apply(simp add: interleave_single_single)
+  apply(rule)+
+  apply(simp add: interleave_right_neutral)
+  done
+
+
+theorem "(
+  (Race2 (Tuple
+    (All2 (Tuple (Pending (Num 1) (Num 0)) (Pending (Num 1) (Num 0))))
+    (All2 (Tuple (Pending (Num 1) (Num 0)) (Pending (Num 2) (Num 0))))
+  )), []) \<Rightarrow>
+  (Resolve (Tuple (Num 1) (Num 2)), [EventResolve (Num 1)]@[EventResolve (Num 2)])
+"
+  apply(rule UF_Race2ResolveI2)
+  apply(rule)+
+  apply(simp add: interleave_left_neutral)
+  apply(rule interleave_Cons_FreeI)
+  apply(rule interleave_Free_ConsI)
+  apply(rule interleave_Nil_NilI)
+  apply(auto)
   done
 end
